Day 3: Restructure & Cleanup

Gaea/Logic/Rules.lean
@@ -11,29 +11,60 @@ namespace Gaea.Logic.Rules
 
 -- Forall
 
-def ForallIntro {P : Sort u} (L : Logic P) (T : Sort v) [LForall P T] := 
+def ForallIntro {P : Sort u} {T : Sort v} (L : Logic P) (Fa : LForall P T) := 
   (f : T -> P) -> ((a : T) -> (L |- f a)) -> (L |- lForall f) 
 
-def ForallElim {P : Sort u} (L : Logic P) (T : Sort v) [LForall P T] := 
+def ForallElim {P : Sort u} {T : Sort v} (L : Logic P) (Fa : LForall P T) := 
   (f : T -> P) -> (L |- lForall f) -> ((a : T) -> (L |- f a))  
+
+-- Exists
+
+def ExistsIntro {P : Sort u} {T : Sort v} (L : Logic P) (X : LExists P T) := 
+  (f : T -> P) -> (a : T) -> (L |- f a) -> (L |- lExists f) 
+
+def ExistsElim {P : Sort u} {T : Sort v} (L : Logic P) (X : LExists P T) := 
+  (f : T -> P) -> (p : P) -> (L |- lExists f) -> 
+    ((a : T) -> (L |- f a) -> (L |- p)) -> (L |- p)
 
 -- If
 
-def IfIntro {P : Sort u} (L : Logic P) [LIf P] := 
+def IfIntro {P : Sort u} (L : Logic P) (If : LIf P) := 
   (p q : P) -> ((L |- p) -> (L |- q)) -> (L |- p -> q) 
 
-def IfElim {P : Sort u} (L : Logic P) [LIf P] := 
+def IfElim {P : Sort u} (L : Logic P) (If : LIf P) := 
   (p q : P) -> (L |- p -> q) -> ((L |- p) -> (L |- q))  
+
+-- Iff
+
+def IfFIntro {P : Sort u} (L : Logic P) (Iff : LIff P) (If : LIf P) := 
+  (p q : P) -> (L |- p -> q) -> (L |- p -> q) -> (L |- p <-> q) 
+
+def IffTo {P : Sort u} (L : Logic P) (Iff : LIff P) (If : LIf P) := 
+  (p q : P) -> (L |- p <-> q) -> (L |- p -> q)  
+
+def IffFrom {P : Sort u} (L : Logic P) (Iff : LIff P) (If : LIf P) := 
+  (p q : P) -> (L |- p <-> q) -> (L |- q -> p)  
+
+-- And
+
+def AndIntro {P : Sort u} (L : Logic P) (And : LAnd P) := 
+  (p q : P) -> (L |- p) -> (L |- q) -> (L |- p /\ q) 
+
+def AndLeft {P : Sort u} (L : Logic P) (And : LAnd P) := 
+  (p q : P) -> (L |- p /\ q) -> (L |- p)  
+
+def AndRight {P : Sort u} (L : Logic P) (And : LAnd P) := 
+  (p q : P) -> (L |- p /\ q) -> (L |- q)  
 
 -- Equality
 
-def EqRefl {P : Sort u} {T : Sort v} (L : Logic P) (C : LEq P T) :=
+def EqRefl {P : Sort u} {T : Sort v} (L : Logic P) (Eq : LEq P T) :=
   (x : T) -> L |- x = x
 
-def EqSymm {P : Sort u} {T : Sort v} (L : Logic P) (C : LEq P T) :=
+def EqSymm {P : Sort u} {T : Sort v} (L : Logic P) (Eq : LEq P T) :=
   (x y : T) -> (L |- x = y) -> (L |- y = x)
 
-def EqTrans {P : Sort u} {T : Sort v} (L : Logic P)  (C : LEq P T) :=
+def EqTrans {P : Sort u} {T : Sort v} (L : Logic P) (Eq : LEq P T) :=
   (x y z : T) -> (L |- x = y) -> (L |- y = z) -> (L |- x = z)
 
 end Gaea.Logic.Rules
