Gaea/Peano/Props.lean
@@ -13,61 +13,116 @@ open Gaea.Syntax
 
 namespace Gaea.Peano.Props
 
+--------------------------------------------------------------------------------
+-- Natural Axioms
+--------------------------------------------------------------------------------
+
 -- Axiom 1
 def natZero {P : Sort u} (T : Type v) [Nat P T] [Zero T] : P :=
   nat (0 : T)
 
 -- Axiom 2
 def eqNatRefl {P : Sort u} (T : Sort v) 
-  [LForall P T] [LIf P] [LEq P T] [Nat P T] : P :=
+  [Nat P T] [LEq P T] [LIf P] [LForall P T] : P :=
   forall (x : T) => nat x -> x = x
 
 -- Axiom 3
 def eqNatSymm {P : Sort u} (T : Sort v) 
-  [LForall P T] [LIf P] [LAnd P] [LEq P T] [Nat P T] : P :=
+  [Nat P T] [LEq P T] [LIf P] [LAnd P] [LForall P T] : P :=
   forall (x y : T) => nat x /\ nat y -> (x = y -> y = x)
 
 -- Axiom 4
 def eqNatTrans {P : Sort u} (T : Sort v) 
-  [LForall P T] [LIf P] [LAnd P] [LEq P T] [Nat P T] : P :=
+  [Nat P T] [LEq P T] [LIf P] [LAnd P] [LForall P T] : P :=
   forall (x y z : T) => nat x /\ nat y /\ nat z -> (x = y /\ y = z -> x = z)
 
 -- Axiom 5
-def natEq {P : Sort u} (L : Logic P) (T : Sort v) 
-  [LForall P T] [LIf P] [LAnd P] [LEq P T] [Nat P T] : P :=
+def natEqNat {P : Sort u} (L : Logic P) (T : Sort v) 
+  [Nat P T] [LEq P T] [LIf P] [LAnd P] [LForall P T] : P :=
   forall (a b : T) => nat b /\ a = b -> nat a
 
 -- Axiom 6
 def natSuccNat {P : Sort u} (T : Sort v) 
-  [LForall P T] [LIf P] [Nat P T] [Succ T] : P :=
+  [Nat P T] [Succ T] [LIf P] [LForall P T] : P :=
   forall (n : T) => nat n -> nat (S n)
 
 -- Axiom 7
-def succNatOto {P : Sort u} (T : Sort v) 
-  [LForall P T] [LIf P] [LAnd P] [LIff P] [LEq P T] [Nat P T] [Succ T] : P :=
+def eqNatIffEqSucc {P : Sort u} (T : Sort v) 
+  [LEq P T] [Succ T] [Nat P T] [LIf P] [LIff P] [LAnd P] [LForall P T] : P :=
   forall (m n : T) => nat m /\ nat n -> (m = n <-> S m = S n)
 
 -- Axiom 7a
-def succNatSubst {P : Sort u} (T : Sort v) 
-  [LForall P T] [LIf P] [LAnd P] [LEq P T] [Nat P T] [Succ T] : P :=
+def eqNatToEqSucc {P : Sort u} (T : Sort v) 
+  [LEq P T] [Succ T] [Nat P T] [LIf P] [LAnd P] [LForall P T] : P :=
   forall (m n : T) => nat m /\ nat n -> (m = n -> S m = S n)
 
 -- Axiom 7b
-def succNatInj {P : Sort u} (T : Sort v) 
-  [LForall P T] [LIf P] [LAnd P] [LEq P T] [Nat P T] [Succ T] : P :=
+def eqSuccToEqNat {P : Sort u} (T : Sort v) 
+  [Nat P T] [LEq P T] [Succ T] [LIf P] [LAnd P] [LForall P T] : P :=
   forall (m n : T) => nat m /\ nat n -> (S m = S n -> m = n)
 
 -- Axiom 8
 def succNatEqZeroFalse {P : Sort u} (T : Type v) 
-  [LForall P T] [LIf P] [LAnd P] [LEq P T] [False P] [Nat P T] [Zero T] [Succ T] : P :=
+  [Nat P T] [LEq P T] [False P] [Zero T] [Succ T] [LIf P] [LAnd P] [LForall P T] : P :=
   forall (m n : T) => nat m /\ nat n -> (S n = 0 -> false)
 
 -- Axiom 9
-def natInduction {P : Sort u} (T : Type v) 
-  [LForall P (T -> P)] [LForall P T] [LIf P] [LAnd P] [LEq P T] 
-  [Nat P T] [Zero T] [Succ T] : P := 
+def natInduction 
+  {P : Sort u} (T : Type v) 
+  [Nat P T] [Zero T] [Succ T]
+  [LIf P] [LAnd P] [LForall P T] [LForall P (T -> P)]  : P := 
   forall (f : T -> P) => 
-    f 0 -> (forall (n : T) => nat n -> (f n -> f (S n))) ->
-      forall (n : T) => nat n -> f n
+    f 0 -> 
+    (forall (n : T) => nat n -> (f n -> f (S n))) ->
+    (forall (n : T) => nat n -> f n)
+
+--------------------------------------------------------------------------------
+-- Addition Axioms
+--------------------------------------------------------------------------------
+
+-- Axiom 1
+def addNatZeroEqNat {P : Sort u} (T : Type v) 
+  [Nat P T] [LEq P T] [Add T] [Zero T] [LIf P] [LForall P T] : P :=
+  forall (a : T) => nat a -> a + 0 = a
+
+-- Axiom 2
+def addNatSuccEqSucc {P : Sort u} (T : Type v) 
+  [Nat P T] [LEq P T] [Add T] [Succ T] [LIf P] [LAnd P] [LForall P T] : P := 
+  forall (a b : T) => nat a /\ nat b -> a + S b = S (a + b)
+
+--------------------------------------------------------------------------------
+-- Multiplication Axioms
+--------------------------------------------------------------------------------
+
+-- Axiom 1
+def mulNatZeroEqZero {P : Sort u} (T : Type v) 
+  [Nat P T] [LEq P T] [Mul T] [Zero T] [LIf P] [LForall P T] : P :=
+  forall (a : T) => nat a -> a * 0 = 0
+
+-- Axiom 2
+def mulNatSuccEqAddMul {P : Sort u} (T : Type v) 
+  [Nat P T] [LEq P T] [Add T] [Mul T] [Succ T] [LIf P] [LAnd P] [LForall P T] : P := 
+  forall (a b : T) => nat a /\ nat b -> a + S b = a + S (a * b)
+
+--------------------------------------------------------------------------------
+-- Inequality Axioms
+--------------------------------------------------------------------------------
+
+-- Axiom 1
+def leIffAddNat 
+  {P : Sort u} (T : Type v) 
+  [Nat P T]  [LE P T] [LEq P T] [Add T] 
+  [LIf P] [LIff P] [LAnd P] [LForall P T] [LExists P T] : P :=
+  forall (a b : T) => nat a /\ nat b -> (a <= b <-> exists c => nat c -> a + c = b)
+
+-- Axiom 2
+def strongNatInduction 
+  {P : Sort u} (T : Type v) 
+  [Nat P T] [LE P T] [Zero T] [Succ T]
+  [LIf P] [LAnd P] [LForall P T] [LForall P (T -> P)] : P := 
+  forall (f : T -> P) => 
+    f 0 -> 
+    (forall (n k : T) => nat n /\ nat k -> (((k <= n) -> f n) -> f (S n))) ->
+    (forall (n : T) => nat n -> f n)
 
 end Gaea.Peano.Props
