Gaea/Peano/Rules.lean
@@ -18,62 +18,67 @@ namespace Gaea.Peano.Rules
 --------------------------------------------------------------------------------
 
 -- Axiom 1
-def NatZero {P : Sort u} (L : Logic P) (T : Type v) [Zero T] [Nat P T] :=
+def NatZero  {P : Sort u} {T : Type v} 
+  (L : Logic P) (N : Nat P T) (Z : Zero T) :=
   L |- nat (0 : T)
 
 -- Axiom 2
-def EqNatRefl {P : Sort u} (L : Logic P) (T : Sort v) [Nat P T] [LEq P T] :=
+def EqNatRefl {P : Sort u} {T : Sort v} 
+  (L : Logic P) (N : Nat P T) (Eq : LEq P T) :=
   (x : T) -> (L |- nat x) -> (L |- x = x)
 
 -- Axiom 3
-def EqNatSymm {P : Sort u} (L : Logic P) (T : Sort v) [Nat P T] [LEq P T] :=
+def EqNatSymm {P : Sort u} {T : Sort v} 
+  (L : Logic P) (N : Nat P T) (Eq : LEq P T) :=
   (x y : T) -> (L |- nat x) -> (L |- nat y) ->
     (L |- x = y) -> (L |- y = x)
 
 -- Axiom 4
-def EqNatTrans {P : Sort u} (L : Logic P) (T : Sort v) [Nat P T] [LEq P T] :=
+def EqNatTrans {P : Sort u} {T : Sort v} 
+  (L : Logic P) (N : Nat P T) (Eq : LEq P T) :=
   (x y z : T) -> (L |- nat x) -> (L |- nat y) -> (L |- nat z) -> 
     (L |- x = y) -> (L |- y = z) -> (L |- x = z)
 
 -- Axiom 5
-def NatEq {P : Sort u} (L : Logic P) (T : Sort v) [Nat P T] [LEq P T] :=
+def NatEqNat {P : Sort u} {T : Sort v} 
+  (L : Logic P) (N : Nat P T) (Eq : LEq P T) :=
   (a b : T) -> (L |- nat b) -> (L |- a = b) -> (L |- nat a)
 
 -- Axiom 6
-def NatSuccNat {P : Sort u} (L : Logic P) (T : Sort v) [Nat P T] [Succ T]:=
+def NatSuccNat {P : Sort u} {T : Sort v} 
+  (L : Logic P) (N : Nat P T) (Su : Succ T) :=
   (n : T) -> (L |- nat n) -> (L |- nat (S n))
 
 -- Axiom 7a
-def SuccNatSubst 
-  {P : Sort u} (L : Logic P) (T : Sort v) [Nat P T] [LEq P T] [Succ T]  :=
+def EqNatToEqSucc {P : Sort u} {T : Sort v} 
+  (L : Logic P) (N : Nat P T) (Eq : LEq P T) (Su : Succ T) :=
   (m n : T) -> (L |- nat m) -> (L |- nat n) -> 
     (L |- m = n) -> (L |- S m = S n)
 
 -- Axiom 7b
-def SuccNatInj 
-  {P : Sort u} (L : Logic P) (T : Sort v) [Nat P T] [LEq P T] [Succ T] :=
+def EqSuccToEqNat {P : Sort u} {T : Sort v} 
+  (L : Logic P) (N : Nat P T) (Eq : LEq P T) (Su : Succ T) :=
   (m n : T) -> (L |- nat m) -> (L |- nat n) -> 
     (L |- S m = S n) -> (L |- m = n)
 
 -- Axiom 8
-def SuccNatEqZeroFalse 
-  {P : Sort u} (L : Logic P) (T : Type v) 
-  [Nat P T] [LEq P T] [Succ T] [Zero T] [False P] :=
+def SuccNatEqZeroFalse {P : Sort u} {T : Type v} 
+  (L : Logic P) (N : Nat P T) (Eq : LEq P T) (Z : Zero T) (Su : Succ T) [False P] :=
   (m n : T) -> (L |- nat m) -> (L |- nat n) -> 
     (L |- S n = 0) -> (L |- false)
 
 -- Axiom 9
 -- Induction over predicates
-def NatInduction 
-  {P : Sort u} (L : Logic P) (T : Type v) [Nat P T] [Zero T] [Succ T] := 
+def NatInduction {P : Sort u} {T : Type v} 
+  (L : Logic P) (N : Nat P T) (Z : Zero T) (Su : Succ T) := 
   (f : T -> P) -> (L |- f 0) -> 
   ((n : T) -> (L |- nat n) -> (L |- f n) -> (L |- f (S n))) ->
   ((n : T) -> (L |- nat n) -> (L |- f n))
 
 -- Axiom 9 (Alt)
 -- Induction over schemas
-def NatInduction'
-  {P : Sort u} (L : Logic P) (T : Type v) [Nat P T] [Zero T] [Succ T] := 
+def NatInduction' {P : Sort u} {T : Type v} 
+  (L : Logic P) (N : Nat P T) (Z : Zero T) (Su : Succ T) := 
   (f : T -> Sort w) -> f 0 ->
   ((n : T) -> (L |- nat n) -> (f n -> f (S n))) ->
   ((n : T) -> (L |- nat n) -> f n)
@@ -83,13 +88,13 @@ def NatInduction'
 --------------------------------------------------------------------------------
 
 -- Axiom 1
-def AddNatZeroEqNat 
-  {P : Sort u} (L : Logic P) (T : Type v) [LEq P T] [Nat P T] [Zero T] [Add T] :=
+def AddNatZeroEqNat {P : Sort u} {T : Type v} 
+  (L : Logic P) (N : Nat P T) (Eq : LEq P T) (A : Add T) (Z : Zero T) :=
   (a : T) -> (L |- nat a) -> (L |- a + 0 = a)
 
 -- Axiom 2
-def AddNatSuccEqSucc 
-  {P : Sort u} (L : Logic P) (T : Type v) [LEq P T] [Nat P T] [Succ T] [Add T] := 
+def AddNatSuccEqSucc {P : Sort u} {T : Type v} 
+  (L : Logic P) (N : Nat P T)  (Eq : LEq P T) (A : Add T) (Su : Succ T) := 
   (a b : T) -> (L |- nat a) -> (L |- nat b) -> (L |- a + S b = S (a + b))
 
 --------------------------------------------------------------------------------
@@ -97,14 +102,13 @@ def AddNatSuccEqSucc
 --------------------------------------------------------------------------------
 
 -- Axiom 1
-def MulNatZeroEqZero 
-  {P : Sort u} (L : Logic P) (T : Type v) [LEq P T] [Nat P T] [Zero T] [Mul T] :=
-  (a b : T) -> (L |- nat a) -> (L |- nat b) -> (L |- a * 0 = 0)
+def MulNatZeroEqZero {P : Sort u} {T : Type v} 
+  (L : Logic P) (N : Nat P T) (Eq : LEq P T) (M : Mul T) (Z : Zero T)  :=
+  (a : T) -> (L |- nat a) -> (L |- a * 0 = 0)
 
 -- Axiom 2
-def MulNatSuccEqAddMul 
-  {P : Sort u} (L : Logic P) (T : Type v) 
-  [LEq P T] [Nat P T] [Succ T] [Add T] [Mul T] := 
+def MulNatSuccEqAddMul {P : Sort u} {T : Type v} 
+  (L : Logic P) (N : Nat P T) (Eq : LEq P T) (M : Mul T) (A : Add T) (Su : Succ T) := 
   (a b : T) -> (L |- nat a) -> (L |- nat b) -> (L |- a + S b = a + S (a * b))
 
 end Gaea.Peano.Rules
