Gaea/Peano.lean
@@ -1,2 +1,1 @@
 import Gaea.Peano.Nat
-import Gaea.Peano.Modules
