Gaea/Peano/Theorems.lean
@@ -6,6 +6,7 @@ import Gaea.Peano.Rules
 
 universes u v w
 
+open Gaea.Logic
 open Gaea.Syntax
 open Gaea.Logic.Rules
 open Gaea.Peano.Rules
@@ -17,9 +18,9 @@ namespace Gaea.Peano
 --------------------------------------------------------------------------------
 
 def natCases 
-{P : Sort u} {L : Logic P} {T : Type v} 
-[Nat P T] [Zero T] [Succ T]
-(natInduction : NatInduction L T)
+{P : Sort u} {T : Type v} {L : Logic P} 
+[Z : Zero T] [Su : Succ T] [N : Nat P T] 
+(natInduction : NatInduction L N Z Su)
 : (f : T -> P) -> 
   (L |- f 0) -> ((n : T) -> (L |- nat n) -> (L |- f (S n))) -> 
     ((n : T) -> (L |- nat n) -> (L |- f n))
@@ -34,18 +35,18 @@ def natCases
 --------------------------------------------------------------------------------
 
 theorem addZeroEqZero 
-{P : Sort u} {L : Logic P} {T : Type v} 
-[LEq P T] [Nat P T] [Zero T] [Add T] 
-(nat_0 : NatZero L T) 
-(An0_eq_n : AddNatZeroEqNat L T)
+{P : Sort u} {T : Type v} {L : Logic P}
+[Eq : LEq P T] [A : Add T] [Z : Zero T] [N : Nat P T]
+(nat_0 : NatZero L N Z) 
+(An0_eq_n : AddNatZeroEqNat L N Eq A Z)
 : L |- 0 + 0 = (0 : T) 
 := An0_eq_n 0 nat_0
 
 theorem natAddNatZero
-{P : Sort u} {L : Logic P} {T : Type v} 
-[LEq P T] [Nat P T] [Zero T] [Add T] 
-(natEq : NatEq L T) 
-(An0_eq_n : AddNatZeroEqNat L T)
+{P : Sort u} {T : Type v} {L : Logic P}
+[Eq : LEq P T] [A : Add T] [Z : Zero T] [N : Nat P T] 
+(natEq : NatEqNat L N Eq) 
+(An0_eq_n : AddNatZeroEqNat L N Eq A Z)
 : (a : T) -> (L |- nat a) -> (L |- nat (a + 0))
 := by
   intro a nat_a
@@ -53,18 +54,19 @@ theorem natAddNatZero
   exact An0_eq_n a nat_a
 
 -- Uses standard (predicate) induction
-theorem NatAddNat_induct
-{P : Sort u} {L : Logic P} {T : Type v} 
-[LForall P T] [LIf P] [LEq P T] [Nat P T] [Zero T] [Succ T] [Add T]
-(ifIntro : IfIntro L)
-(ifElim : IfElim L)
-(forallIntro : ForallIntro L T)
-(forallElim : ForallElim L T)
-(nat_S : NatSuccNat L T) 
-(natEq : NatEq L T) 
-(natInduction : NatInduction L T)
-(An0_eq_n : AddNatZeroEqNat L T)
-(AnS_eq_S : AddNatSuccEqSucc L T)
+theorem natAddNat_induct
+{P : Sort u} {T : Type v} {L : Logic P}
+[N : Nat P T] [Eq : LEq P T] [A : Add T] [Z : Zero T] [Su : Succ T] 
+[Fa : LForall P T] [If : LIf P] 
+(ifIntro : IfIntro L If)
+(ifElim : IfElim L If)
+(forallIntro : ForallIntro L Fa)
+(forallElim : ForallElim L Fa)
+(natEq : NatEqNat L N Eq) 
+(nat_S : NatSuccNat L N Su) 
+(natInduction : NatInduction L N Z Su)
+(An0_eq_n : AddNatZeroEqNat L N Eq A Z)
+(AnS_eq_S : AddNatSuccEqSucc L N Eq A Su)
 : (b : T) -> (L |- nat b) -> (L |- forall (a : T) => nat a -> nat (a + b))
 := by
   intro b nat_b
@@ -75,43 +77,44 @@ theorem NatAddNat_induct
   apply ifIntro; intro nat_a
   exact natAddNatZero natEq An0_eq_n a nat_a
   -- Induction
-  intro a nat_a p_ih
+  intro a nat_a p_Nn_to_NAna
   apply forallIntro; intro b
   apply ifIntro; intro nat_b
-  have nat_Aba := ifElim _ _ (forallElim _ p_ih b) nat_b 
-  have abSa_eq_Saba := AnS_eq_S _ _ nat_b nat_a
+  have nat_Aba := ifElim _ _ (forallElim _ p_Nn_to_NAna b) nat_b 
+  have AbSa_eq_SAba := AnS_eq_S _ _ nat_b nat_a
   have nat_SAba := nat_S _ nat_Aba
-  exact natEq _ _ nat_SAba abSa_eq_Saba
+  exact natEq _ _ nat_SAba AbSa_eq_SAba
   exact nat_b
 
-theorem NatAddNat
-{P : Sort u} {L : Logic P} {T : Type v} 
-[LForall P T] [LIf P] [LEq P T] [Nat P T] [Zero T] [Succ T] [Add T]
-(ifIntro : IfIntro L)
-(ifElim : IfElim L)
-(forallIntro : ForallIntro L T)
-(forallElim : ForallElim L T)
-(nat_S : NatSuccNat L T) 
-(natEq : NatEq L T) 
-(natInduction : NatInduction L T)
-(An0_eq_n : AddNatZeroEqNat L T)
-(AnS_eq_S : AddNatSuccEqSucc L T)
+theorem natAddNat
+{P : Sort u} {T : Type v} {L : Logic P} 
+[N : Nat P T] [Eq : LEq P T] [A : Add T] [Z : Zero T] [Su : Succ T]
+[Fa : LForall P T] [If : LIf P] 
+(ifIntro : IfIntro L If)
+(ifElim : IfElim L If)
+(forallIntro : ForallIntro L Fa)
+(forallElim : ForallElim L Fa)
+(natEq : NatEqNat L N Eq) 
+(nat_S : NatSuccNat L N Su) 
+(natInduction : NatInduction L N Z Su)
+(An0_eq_n : AddNatZeroEqNat L N Eq A Z)
+(AnS_eq_S : AddNatSuccEqSucc L N Eq A Su)
 : (a b : T) -> (L |- nat a) -> (L |- nat b) -> (L |- nat (a + b))
 := by
   intro a b nat_a nat_b
-  have h :=  NatAddNat_induct ifIntro ifElim forallIntro forallElim  
-    nat_S natEq natInduction An0_eq_n AnS_eq_S b nat_b
+  have h :=  natAddNat_induct ifIntro ifElim forallIntro forallElim  
+    natEq nat_S natInduction An0_eq_n AnS_eq_S b nat_b
   exact ifElim _ _ (forallElim _ h a) nat_a
 
 -- Uses schema induction
-theorem NatAddNat'
-{P : Sort u} {L : Logic.{u,w} P} {T : Type v} 
-[LEq P T] [Nat P T] [Zero T] [Succ T] [Add T]
-(nat_S : NatSuccNat L T) 
-(natEq : NatEq L T) 
-(natInduction : NatInduction'.{u,v,(imax (v+1) w)} L T)
-(An0_eq_n : AddNatZeroEqNat L T)
-(AnS_eq_S : AddNatSuccEqSucc L T)
+theorem natAddNat'
+{P : Sort u} {T : Type v} {L : Logic.{u,w} P}
+[N : Nat P T] [Eq : LEq P T]  [A : Add T] [Z : Zero T] [Su : Succ T] 
+(natEq : NatEqNat L N Eq) 
+(nat_S : NatSuccNat L N Su) 
+(natInduction : NatInduction'.{u,v,(imax (v+1) w)} L N Z Su)
+(An0_eq_n : AddNatZeroEqNat L N Eq A Z)
+(AnS_eq_S : AddNatSuccEqSucc L N Eq A Su)
 : (a b : T) -> (L |- nat a) -> (L |- nat b) -> (L |- nat (a + b))
 := by
   intro m n nat_m nat_n
