Gaea/Syntax/Math.lean
@@ -1,9 +1,19 @@
 namespace Gaea.Syntax
 
+-- Numerics
+
 abbrev Zero (N : Type u) 
   := OfNat N (natLit! 0)
 
 class Succ (N : Sort u) :=
   (S : N -> N)
+
+-- Inequalities
+
+class LT (P : Sort u) (N : Sort v) :=
+  (lt : N -> N -> P)
+
+class LE (P : Sort u) (N : Sort v)  :=
+  (le : N -> N -> P)
 
 end Gaea.Syntax
